README.md
@@ -138,8 +138,7 @@ All the Coq code is in [`nola/`](nola/) and structured as follows:
     * [`prod`](nola/examples/rust_halt/prod.v) (Product type),
       [`sum`](nola/examples/rust_halt/sum.v) (Sum type)
     * [`rec`](nola/examples/rust_halt/rec.v) (Recursive type),
-      [`mod`](nola/examples/rust_halt/mod.v) (Modification type),
-      [`anydep`](nola/examples/rust_halt/anydep.v) (Any-depth type)
+      [`mod`](nola/examples/rust_halt/mod.v) (Modification type)
     * [`ptr`](nola/examples/rust_halt/ptr.v) (Utility for pointer types),
       [`box`](nola/examples/rust_halt/box.v) (Box pointer type),
       [`shrref`](nola/examples/rust_halt/shrref.v) (Shared reference type),
